Manual/BasicTypes.lean
@@ -11,6 +11,7 @@ import Manual.BasicTypes.Nat
 import Manual.BasicTypes.Int
 import Manual.BasicTypes.String
 import Manual.BasicTypes.Array
+import Manual.BasicTypes.ByteArray
 import Manual.BasicTypes.Fin
 import Manual.BasicTypes.UInt
 import Manual.BasicTypes.BitVec
@@ -315,6 +316,8 @@ Most comparisons on Booleans should be performed using the {inst}`DecidableEq Bo
 {include 0 Manual.BasicTypes.List}
 
 {include 0 Manual.BasicTypes.Array}
+
+{include 0 Manual.BasicTypes.ByteArray}
 
 {include 0 Manual.BasicTypes.Maps}
 
