Manual/BasicTypes/String/RawPos.lean
@@ -1,0 +1,85 @@
+/-
+Copyright (c) 2024 Lean FRO LLC. All rights reserved.
+Released under Apache 2.0 license as described in the file LICENSE.
+Author: David Thrane Christiansen
+-/
+
+import VersoManual
+
+import Manual.Meta
+open Manual.FFIDocType
+
+open Verso.Genre Manual
+open Verso.Genre.Manual.InlineLean
+
+set_option pp.rawOnError true
+
+#doc (Manual) "Raw Positions" =>
+%%%
+tag := "string-api-pos"
+%%%
+
+
+{docstring String.Pos.Raw}
+
+# Validity
+
+{docstring String.Pos.Raw.isValid}
+
+{docstring String.Pos.Raw.isValidForSlice}
+
+# Boundaries
+
+{docstring String.endPos}
+
+{docstring String.Pos.Raw.atEnd}
+
+# Comparisons
+
+{docstring String.Pos.Raw.min}
+
+{docstring String.Pos.Raw.byteDistance}
+
+{docstring String.Pos.Raw.substrEq}
+
+# Adjustment
+
+{docstring String.Pos.Raw.prev}
+
+{docstring String.Pos.Raw.next}
+
+{docstring String.Pos.Raw.next'}
+
+{docstring String.Pos.Raw.nextUntil}
+
+{docstring String.Pos.Raw.nextWhile}
+
+{docstring String.Pos.Raw.inc}
+
+{docstring String.Pos.Raw.increaseBy}
+
+{docstring String.Pos.Raw.offsetBy}
+
+{docstring String.Pos.Raw.dec}
+
+{docstring String.Pos.Raw.decreaseBy}
+
+{docstring String.Pos.Raw.unoffsetBy}
+
+# String Lookups
+
+{docstring String.Pos.Raw.extract}
+
+{docstring String.Pos.Raw.get}
+
+{docstring String.Pos.Raw.get!}
+
+{docstring String.Pos.Raw.get'}
+
+{docstring String.Pos.Raw.get?}
+
+# String Modifications
+
+{docstring String.Pos.Raw.set}
+
+{docstring String.Pos.Raw.modify}
