Manual/Elaboration.lean
@@ -228,7 +228,8 @@ def third_of_five : List α → Option α
 set_option pp.match false
 /--
 info: third_of_five.eq_def.{u_1} {α : Type u_1} (x✝ : List α) :
-  third_of_five x✝ = third_of_five.match_1 (fun x => Option α) x✝ (fun head head x head head => some x) fun x => none
+  third_of_five x✝ =
+    third_of_five.match_1 (fun x => Option α) x✝ (fun head head_1 x head_2 head_3 => some x) fun x => none
 -/
 #check_msgs in
 #check third_of_five.eq_def
