Manual/Meta/Basic.lean
@@ -19,7 +19,7 @@ def parserInputString [Monad m] [MonadFileMap m]
     (str : TSyntax `str) :
     m String := do
   let text ← getFileMap
-  let preString := text.source.extract 0 (str.raw.getPos?.getD 0)
+  let preString := String.Pos.Raw.extract text.source 0 (str.raw.getPos?.getD 0)
   let mut code := ""
   let mut iter := preString.iter
   while !iter.atEnd do
@@ -30,7 +30,7 @@ def parserInputString [Monad m] [MonadFileMap m]
     iter := iter.next
   let strOriginal? : Option String := do
     let ⟨start, stop⟩ ← str.raw.getRange?
-    text.source.extract start stop
+    start.extract text.source stop
   code := code ++ strOriginal?.getD str.getString
   return code
 
@@ -52,7 +52,7 @@ instance : Quote SyntaxError where
 
 -- Based on mkErrorMessage used in Lean upstream - keep them in synch for best UX
 open Lean.Parser in
-private partial def mkSyntaxError (c : InputContext) (pos : String.Pos) (stk : SyntaxStack) (e : Parser.Error) : SyntaxError := Id.run do
+private partial def mkSyntaxError (c : InputContext) (pos : String.Pos.Raw) (stk : SyntaxStack) (e : Parser.Error) : SyntaxError := Id.run do
   let mut pos := pos
   let mut endPos? := none
   let mut e := e
